Fix style

src/StandardLibrary/UInt.dfy
@@ -1,5 +1,6 @@
 module {:extern "STLUInt"} StandardLibrary.UInt {
-  newtype UInt8 = x | 0 <= x < 256
+  const UINT8_LIMIT := 0x100
+  newtype UInt8 = x | 0 <= x < UINT8_LIMIT
 
   const UINT16_LIMIT := 0x1_0000
   newtype UInt16 = x | 0 <= x < UINT16_LIMIT
@@ -14,17 +15,17 @@ module {:extern "STLUInt"} StandardLibrary.UInt {
   function method UInt16ToSeq(x: UInt16): seq<UInt8>
     ensures |UInt16ToSeq(x)| == 2
   {
-    var b0: UInt8 := (x / 256) as UInt8;
-    var b1: UInt8 := (x % 256) as UInt8;
+    var b0: UInt8 := (x / 0x100) as UInt8;
+    var b1: UInt8 := (x % 0x100) as UInt8;
     [b0, b1]
   }
 
   function method SeqToUInt16(p: seq<UInt8>): UInt16
     requires |p| == 2
   {
-    var x1 :=    (p[0] as int) * 256;
-    assert x1 <= 256 * 256;
-    var  x := x1 + (p[1] as int);
+    var x0 := (p[0] as int) * 0x100;
+    assert x0 <= UINT8_LIMIT * 0x100;
+    var x := x0 + (p[1] as int);
     assert x < UINT16_LIMIT;
     x as UInt16
   }
@@ -44,8 +45,8 @@ module {:extern "STLUInt"} StandardLibrary.UInt {
     ensures ret.Length == 2
   {
     ret := new UInt8[2];
-    ret[0] := (x / 256) as UInt8;
-    ret[1] := (x % 256) as UInt8;
+    ret[0] := (x / 0x100) as UInt8;
+    ret[1] := (x % 0x100) as UInt8;
   }
 
   function method arrayToUInt16(p: array<UInt8>): (ret: UInt16)
@@ -53,9 +54,9 @@ module {:extern "STLUInt"} StandardLibrary.UInt {
     requires p.Length == 2
     ensures SeqToUInt16(p[..]) == ret
   {
-    var x1 :=    p[0] as int * 256;
-    assert x1 <= 256 * 256;
-    var  x := x1 + p[1] as int;
+    var x0 := p[0] as int * 0x100;
+    assert x0 <= 0x100 * 0x100;
+    var x := x0 + p[1] as int;
     assert x < UINT16_LIMIT;
     x as UInt16
   }
@@ -64,15 +65,13 @@ module {:extern "STLUInt"} StandardLibrary.UInt {
     ensures |UInt32ToSeq(x)| == 4
   {
     var b0 := ( x / 0x100_0000) as UInt8;
-    var x0: UInt32 :=  x - (b0 as UInt32 * 0x100_0000);
+    var x0: UInt32 := x - (b0 as UInt32 * 0x100_0000);
 
     var b1 := (x0 / 0x1_0000) as UInt8;
     var x1: UInt32 := x0 - (b1 as UInt32 * 0x1_0000);
 
     var b2 := (x1 / 0x100) as UInt8;
-    // or for symmetry:
-    // x2 := x1 - (b2 * 0x100);
-    // b3 := (x2 / 1) as UInt8;
+
     var b3 := (x1 % 0x100) as UInt8;
     [b0, b1, b2, b3]
   }
@@ -80,14 +79,10 @@ module {:extern "STLUInt"} StandardLibrary.UInt {
   function method SeqToUInt32(p: seq<UInt8>): UInt32
     requires |p| == 4
   {
-    // 2^24 = 0x100_0000
-    var x3 :=    p[0] as int * 0x100_0000;
-    // 2^16 = 0x1_0000
-    var x2 := x3 + p[1] as int * 0x1_0000;
-    // 2^8 = 0x100
-    var x1 := x2 + p[2] as int * 0x100;
-    // 2^0 = 0x1
-    var  x := x1 + p[3] as int;
+    var x0 := p[0] as int * 0x100_0000;
+    var x1 := x0 + p[1] as int * 0x1_0000;
+    var x2 := x1 + p[2] as int * 0x100;
+    var x := x2 + p[3] as int;
     assert x < UINT32_LIMIT;
     x as UInt32
   }
@@ -116,9 +111,7 @@ module {:extern "STLUInt"} StandardLibrary.UInt {
     x' := x' - (ret[1] as UInt32 * 0x1_0000);
 
     ret[2] := (x' / 0x100) as UInt8;
-    // or for symmetry:
-    // x' := x' - (ret[2] * 0x100);
-    // ret[3] := (x' / 1) as UInt8;
+
     ret[3] := (x' % 0x100) as UInt8;
   }
 
@@ -127,14 +120,10 @@ module {:extern "STLUInt"} StandardLibrary.UInt {
     requires p.Length == 4
     ensures SeqToUInt32(p[..]) == ret
   {
-    // 2^24 = 0x100_0000
-    var x3 :=    p[0] as int * 0x100_0000;
-    // 2^16 = 0x1_0000
-    var x2 := x3 + p[1] as int * 0x1_0000;
-    // 2^8 = 0x100
-    var x1 := x2 + p[2] as int * 0x100;
-    // 2^0 = 0x1
-    var  x := x1 + p[3] as int;
+    var x0 := p[0] as int * 0x100_0000;
+    var x1 := x0 + p[1] as int * 0x1_0000;
+    var x2 := x1 + p[2] as int * 0x100;
+    var x := x2 + p[3] as int;
     assert x < UINT32_LIMIT;
     x as UInt32
   }
